src/Assembly/Syntax.v
@@ -18,10 +18,34 @@ Local Set Implicit Arguments.
 Local Set Primitive Projections.
 
 Inductive REG :=
+(* XMM/YMM/ZMM registers *)
+| zmm0  | zmm1  | zmm2  | zmm3  | zmm4  | zmm5  | zmm6  | zmm7  | zmm8  | zmm9  | zmm10  | zmm11  | zmm12  | zmm13  | zmm14  | zmm15 | zmm16 | zmm17 | zmm18 | zmm19 | zmm20 | zmm21 | zmm22 | zmm23 | zmm24 | zmm25 | zmm26  | zmm27  | zmm28  | zmm29  | zmm30  | zmm31
+| ymm0  | ymm1  | ymm2  | ymm3  | ymm4  | ymm5  | ymm6  | ymm7  | ymm8  | ymm9  | ymm10  | ymm11  | ymm12  | ymm13  | ymm14  | ymm15
+| xmm0  | xmm1  | xmm2  | xmm3  | xmm4  | xmm5  | xmm6  | xmm7  | xmm8  | xmm9  | xmm10  | xmm11  | xmm12  | xmm13  | xmm14  | xmm15
+(* Segment registers *)
+| cs | ds | es | fs | gs | ss
+(* Control registers *)
+| cr0 | cr1 | cr2 | cr3 | cr4 | cr8 | cr9 | cr10 | cr11 | cr12 | cr13 | cr14 | cr15
+| msw
+| mxcsr
+(* Debug registers *)
+| dr0 | dr1 | dr2 | dr3 | dr4 | dr5 | dr6 | dr7 | dr8 | dr9 | dr10 | dr11 | dr12 | dr13 | dr14 | dr15
+(* General purpose registers (64/32/16/8 bit) *)
 |     rax |     rcx |     rdx |     rbx | rsp  | rbp  | rsi  | rdi  | r8  | r9  | r10  | r11  | r12  | r13  | r14  | r15  | rip
 |     eax |     ecx |     edx |     ebx | esp  | ebp  | esi  | edi  | r8d | r9d | r10d | r11d | r12d | r13d | r14d | r15d | eip
 |      ax |      cx |      dx |      bx |  sp  |  bp  |  si  |  di  | r8w | r9w | r10w | r11w | r12w | r13w | r14w | r15w | ip
 | ah | al | ch | cl | dh | dl | bh | bl |  spl |  bpl |  sil |  dil | r8b | r9b | r10b | r11b | r12b | r13b | r14b | r15b
+(* MMX registers *)
+| mm0 | mm1 | mm2 | mm3 | mm4 | mm5 | mm6 | mm7
+(* Special registers *)
+| st0 | st1 | st2 | st3 | st4 | st5 | st6 | st7  (* FPU stack registers*)
+| k0 | k1 | k2 | k3 | k4 | k5 | k6 | k7          (* AVX-512 mask registers *)
+| gdtr | idtr | ldtr | tr
+| cw | sw | tw | fp_cs | fp_opc | fp_ds
+(* Flags registers *)
+(* | rflags
+| eflags
+| flags *)
 .
 
 Derive REG_Listable SuchThat (@FinitelyListable REG REG_Listable) As REG_FinitelyListable.
@@ -35,7 +59,7 @@ Definition REG_eq_dec : forall x y : REG, {x = y} + {x <> y} := eq_dec_of_listab
 Definition CONST := Z.
 Coercion CONST_of_Z (x : Z) : CONST := x.
 
-Inductive AccessSize := byte | word | dword | qword.
+Inductive AccessSize := byte | word | dword | qword | tbyte | xmmword | ymmword | zmmword.
 
 Derive AccessSize_Listable SuchThat (@FinitelyListable AccessSize AccessSize_Listable) As AccessSize_FinitelyListable.
 Proof. prove_ListableDerive. Qed.
@@ -51,6 +75,10 @@ Coercion bits_of_AccessSize (x : AccessSize) : N
      | word => 16
      | dword => 32
      | qword => 64
+     | tbyte => 80
+     | xmmword => 128
+     | ymmword => 256
+     | zmmword => 512
      end.
 
 Record MEM := { mem_bits_access_size : option AccessSize ; mem_base_reg : option REG ; mem_scale_reg : option (Z * REG) ; mem_base_label : option string ; mem_offset : option Z }.
@@ -102,6 +130,10 @@ Inductive OpCode :=
 | dw
 | dd
 | dq
+| dt
+| do
+| dy
+| dz
 | dec
 | imul
 | inc
@@ -176,6 +208,10 @@ Definition accesssize_of_declaration (opc : OpCode) : option AccessSize :=
   | dd => Some dword
   | dq => Some qword
   | dw => Some word
+  | dt => Some tbyte
+  | do => Some xmmword
+  | dy => Some ymmword
+  | dz => Some zmmword
   | adc
   | adcx
   | add
@@ -276,14 +312,38 @@ Definition Lines := list Line.
 
 Definition reg_size (r : REG) : N :=
       match r with
+      |(xmm0 | xmm1 | xmm2 | xmm3 | xmm4 | xmm5 | xmm6 | xmm7 | xmm8 | xmm9 | xmm10 | xmm11 | xmm12 | xmm13 | xmm14 | xmm15)
+       => 128
+      |(zmm0 | zmm1 | zmm2 | zmm3 | zmm4 | zmm5 | zmm6 | zmm7 | zmm8 | zmm9 | zmm10 | zmm11 | zmm12 | zmm13 | zmm14 | zmm15 | zmm16 | zmm17 | zmm18 | zmm19 | zmm20 | zmm21 | zmm22 | zmm23 | zmm24 | zmm25 | zmm26  | zmm27  | zmm28  | zmm29  | zmm30  | zmm31)
+       => 512
+      |(ymm0 | ymm1 | ymm2 | ymm3 | ymm4 | ymm5 | ymm6 | ymm7 | ymm8 | ymm9 | ymm10 | ymm11 | ymm12 | ymm13 | ymm14 | ymm15)
+       => 256
       |(    rax |     rcx |     rdx |     rbx | rsp  | rbp  | rsi  | rdi  | r8  | r9  | r10  | r11  | r12  | r13  | r14  | r15  | rip)
        => 64
       |(    eax |     ecx |     edx |     ebx | esp  | ebp  | esi  | edi  | r8d | r9d | r10d | r11d | r12d | r13d | r14d | r15d | eip)
        => 32
       |(     ax |      cx |      dx |      bx |  sp  |  bp  |  si  |  di  | r8w | r9w | r10w | r11w | r12w | r13w | r14w | r15w | ip)
        => 16
+      |(cs | ds | es | fs | gs | ss)
+       => 16
       |(ah | al | ch | cl | dh | dl | bh | bl |  spl |  bpl |  sil |  dil | r8b | r9b | r10b | r11b | r12b | r13b | r14b | r15b)
        => 8
+      |(cr0 | cr1 | cr2 | cr3 | cr4 | cr8 | cr9 | cr10 | cr11 | cr12 | cr13 | cr14 | cr15)
+       => 64
+      |(dr0 | dr1 | dr2 | dr3 | dr4 | dr5 | dr6 | dr7 | dr8 | dr9 | dr10 | dr11 | dr12 | dr13 | dr14 | dr15)
+       => 64
+      |(mm0 | mm1 | mm2 | mm3 | mm4 | mm5 | mm6 | mm7)
+       => 64
+      |(st0 | st1 | st2 | st3 | st4 | st5 | st6 | st7)
+       => 80
+      |(k0 | k1 | k2 | k3 | k4 | k5 | k6 | k7)
+       => 64
+      |(gdtr | idtr | ldtr | tr)
+       => 16
+      |(cw | sw | tw | fp_cs | fp_opc | fp_ds)
+       => 16
+      | msw => 16
+      | mxcsr => 32
       end.
 
 Definition standalone_operand_size (x : ARG) : option N :=
@@ -355,6 +415,25 @@ Definition widest_register_of (r : REG) : REG :=
   | (r14b | r14w | r14d | r14) => r14
   | (r15b | r15w | r15d | r15) => r15
   | (ip | eip | rip) => rip
+  (* | (flags | eflags | rflags) => rflags *)
+  | (xmm0 | ymm0 | zmm0) => zmm0
+  | (xmm1 | ymm1 | zmm1) => zmm1
+  | (xmm2 | ymm2 | zmm2) => zmm2
+  | (xmm3 | ymm3 | zmm3) => zmm3
+  | (xmm4 | ymm4 | zmm4) => zmm4
+  | (xmm5 | ymm5 | zmm5) => zmm5
+  | (xmm6 | ymm6 | zmm6) => zmm6
+  | (xmm7 | ymm7 | zmm7) => zmm7
+  | (xmm8 | ymm8 | zmm8) => zmm8
+  | (xmm9 | ymm9 | zmm9) => zmm9
+  | (xmm10 | ymm10 | zmm10) => zmm10
+  | (xmm11 | ymm11 | zmm11) => zmm11
+  | (xmm12 | ymm12 | zmm12) => zmm12
+  | (xmm13 | ymm13 | zmm13) => zmm13
+  | (xmm14 | ymm14 | zmm14) => zmm14
+  | (xmm15 | ymm15 | zmm15) => zmm15
+  | (msw | cr0) => cr0
+  | _ => r
   end.
 
 Definition widest_registers := Eval lazy in List.filter (fun x => REG_beq x (widest_register_of x)) (list_all REG).
